$$f(x) = -2\sin(x+1) + \sin(x+2) + 2\sin(-3x) + \sin(-x) + 2\cos(-3x+2) + 1.$$



$$f(x) = -2\sin(-3x+1) - 2\sin(-x+1) + 2\sin(-x+2) + 2\sin(3x+2) + \cos(x) + 1.$$



$$f(x) = -\sin(x+2) - \sin(2x+1) - \sin(-2x) + 2\sin(3x) - 2\cos(-3x+1) + 1$$



$$f(x) = -\sin(-3x) + \sin(3x) + 2\cos(-3x+1) + 2\cos(3x+2) - \cos(3x) + 1.$$



$$f(x) = \sin(-x+2) - 2\sin(x) - \cos(x+2) + \cos(2x+2) + \cos(3x+2) + 1.$$



$$f(x) = \sin\left(-2x+1\right) - 2\,\sin\left(-x\right) + \cos\left(2x+2\right) - \cos\left(-x\right) + 2\,\cos\left(x\right) + 1.$$



$$f(x) = -\sin(x+1) - \sin(x+2) + \sin(x) - \cos(3x+1) + \cos(2x) + 1.$$



$$f(x) = -\sin(-x+2) + 2\sin(x+1) + 2\sin(2x+2) - \cos(-x+2) - \cos(x+1) + 1$$



$$f(x) = \sin\left(-2x+1\right) + \sin\left(-x+2\right) + \sin\left(-x\right) - \cos\left(x+1\right) + 2\cos\left(2x+2\right) + 1.$$



$$f(x) = \sin(-x+2) + \cos(-2x+1) - \cos(x+1) + \cos(3x) + 1$$



$$f(x) = -2\sin(-3x+2) + 3\sin(-x+2) + \sin(3x+1) - 2\sin(-x) + 1.$$



$$f(x) = 2\sin(-2x+2) - 2\sin(x+1) + \sin(x+2) + 2\cos(x+2) + 2\cos(2x+2) + 1.$$



$$f(x) = -2\sin(-3x+2) - \sin(-2x+2) - 2\sin(x+2) + \sin(3x+2) + 2\cos(-3x+1) + 1$$



$$f(x) = \sin(-x) + \sin(x) + \cos(-x+1) + 2\cos(x+1) + 1.$$



$$f(x) = \cos\left(-3x+2\right) + 2\,\cos\left(-x+1\right) + \cos\left(-x+2\right) + 1.$$



$$f(x) = \sin(-2x+2) + \sin(-x+2) + \sin(-3x) + \cos(2x+2) - \cos(-2x) + 1.$$



$$f(x) = \sin(2x+1) - 2\sin(-x) - 2\cos(2x) + 1.$$



$$f(x) = \sin(x) - \cos(-x+1) - \cos(3x) + 1$$



$$f(x) = \sin(2x+2) + 2\sin(-3x) - 2\cos(-x+1) - 2\cos(3x+2) + \cos(-x) + 1.$$



$$f(x) = \sin\left(-2x+2\right) - \sin\left(3x+1\right) + \sin\left(3x+2\right) - \sin\left(3x\right) + \cos\left(-3x+1\right) + 1$$



$$f(x) = -2\sin(-x+2) - 2\cos(-2x+1) - \cos(-x+2) + 1.$$



$$f(x) = -2\sin(-x+2) - \sin(x+2) + \cos(-x+2) - \cos(3x) + 2\cos(x) + 1.$$



$$f(x) = 2\sin(-3x+2) - \sin(x+1) - 2\sin(3x+1) - \sin(3x) - \cos(-x+2) + 1.$$



$$f(x) = \sin(-x+1) + 2\sin(x+1) + \sin(x+2) - 2\sin(-x) + 2\cos(x+1) + 1.$$



$$f(x) = \sin(3x+2) - 2\sin(x) - \cos(-x+2) + 1.$$



$$f(x) = \sin(-x+1) + 2\sin(-x+2) - \sin(3x+1) + 1.$$



$$f(x) = -2\sin(3x+1) - \cos(-3x+1) - \cos(3x+2) + 1$$



$$f(x) = 2\sin(x+1) + \sin(3x) - \sin(x) + 2\cos(-2x+2) + \cos(2x+2) + 1.$$



$$f(x) = \sin\left(-3x+1\right) - 2\,\cos\left(3x+1\right) + \cos\left(3x\right) + 1.$$



$$f(x) = -\sin\left(-2x+1\right) + \cos\left(x+1\right) + \cos\left(x+2\right) + \cos\left(2x+1\right) - \cos\left(-2x\right) + 1.$$



$$f(x) = -2\sin(-x+2) + 2\sin(x+2) + \sin(x) - 2\cos(-3x+1) - \cos(3x+1) + 1.$$



$$f(x) = \sin\left(-3x+2\right) + 2\,\sin\left(-x+2\right) - \cos\left(x+1\right) + 4\,\cos\left(x+2\right) + 1.$$



$$f(x) = -2\sin(x+1) + 2\cos(-2x+2) + \cos(x+1) + \cos(-x) + \cos(2x) + 1.$$



$$f(x) = -2\sin(-x+2) - \cos(-2x) + \cos(2x) + \cos(3x) + 1.$$



$$f(x) = -\sin(-3x) + \cos(-3x+2) + \cos(x+1) + \cos(x+2) + \cos(3x+2) + 1.$$



$$f(x) = -\sin(-2x) + 3\cos(x) + 1$$


$$f(x) = -2\sin(2x+2) - 2\cos(-2x+2) + \cos(-x+1) + \cos(3x+1) + \cos(-2x) + 1.$$



$$f(x) = \sin\left(-3x+1\right) - \cos\left(x+1\right) - \cos\left(x+2\right) + 1.$$



$$f(x) = -\sin(3x+1) + 2\sin(3x+2) + 2\sin(3x) - \cos(-x+2) - 2\cos(x+1) + 1.$$



$$f(x) = -\sin(-x+2) - \cos(-x+2) - \cos(-2x) + 2\cos(2x) + 1.$$



$$f(x) = -\sin(-x+2) - \sin(x+2) - \sin(-x) - \cos(-2x+2) + \cos(2x) + 1.$$



$$f(x) = 2\cos(-3x+1) - \cos(-3x+2) - 2\cos(-3x) + 2\cos(3x) - \cos(x) + 1.$$



$$f(x) = -\sin(2x+1) + 2\cos(-2x+1) + \cos(2x+1) + \cos(3x+1) - \cos(2x) + 1.$$



$$f(x) = \sin(-x+1) - \sin(2x+1) + \sin(-2x) + 2\sin(x) + 2\cos(-2x) + 1$$



$$f(x) = -\sin(3x+2) - 2\sin(-x) + \cos(x+2) - \cos(2x+2) + \cos(3x+1) + 1.$$



$$f(x) = \sin(x+2) - 2\sin(2x+1) - \sin(-x) - \cos(-x+2) - 2\cos(x) + 1$$



$$f(x) = -\sin(x+2) - 2\cos(-3x+1) + \cos(-x+2) - \cos(x+1) - 2\cos(3x+2) + 1.$$



$$f(x) = -\sin(x+2) + 2\cos(-x+2) + \cos(2x+1) - \cos(-x) + 2\cos(x) + 1.$$



$$f(x) = \sin\left(-3x+2\right) - \sin\left(3x+1\right) - 2\cos\left(-2x+1\right) + \cos\left(-2x+2\right) + \cos\left(2x+2\right) + 1.$$



$$f(x) = -\sin\left(-2x+2\right) - 2\sin\left(-2x\right) + 2\cos\left(2x+1\right) + 1.$$



$$f(x) = 2\sin(-x) + 2\sin(x) - \cos(x+2) + \cos(3x+1) - \cos(-3x) + 1.$$



$$f(x) = \sin(2x+1) - 2\sin(x) - 2\cos(x+1) + \cos(-3x) + 1.$$



$$f(x) = -2\sin(-x+2) - \sin(3x) - \cos(3x+1) + \cos(-2x) + 2\cos(x) + 1$$



$$f(x) = \cos(-3x+1) - 2\cos(-x+1) - \cos(x+1) - \cos(x+2) - \cos(x) + 1.$$



$$f(x) = -\sin(x) - \cos(-2x+1) - \cos(2x) + 1.$$



$$f(x) = -\sin\left(-2x+2\right) + 2\sin\left(-x+1\right) - \cos\left(x+1\right) + \cos\left(-3x\right) + 1.$$



$$f(x) = \sin(-x+1) + \sin(x+1) + 2\sin(2x+1) - \cos(-2x+1) + \cos(2x) + 1.$$



$$f(x) = -\sin(x+2) + \sin(2x+1) - \cos(-3x+2) - \cos(2x+1) - \cos(3x+2) + 1.$$



$$f(x) = \sin(-x+1) - \sin(x+2) + \sin(2x+1) + 2\cos(x+2) - \cos(-2x) + 1.$$



$$f(x) = \sin(-x+2) - 2\sin(x+1) + \sin(x) + \cos(-3x+2) + \cos(-2x) + 1.$$



$$f(x) = \sin(3x+1) + 2\sin(2x) - \cos(-2x+2) + \cos(-x+2) - \cos(3x) + 1.$$



$$f(x) = -\sin\left(-3x+1\right) + \cos\left(x+2\right) + \cos\left(3x+1\right) + 2\cos\left(-x\right) - 2\cos\left(x\right) + 1.$$



$$f(x) = \sin(-2x+2) - \sin(-x+1) - \sin(3x+1) - 2\sin(2x) + \cos(-2x+2) + 1$$



$$f(x) = -\sin\left(-2x+1\right) + \sin\left(2x+1\right) - \sin\left(x\right) - \cos\left(-2x+1\right) + 2\cos\left(-2x+2\right) + 1.$$



$$f(x) = \sin(-3x+2) + 2\sin(-x+1) - 2\sin(-x+2) - \sin(x+1) + 2\sin(-x) + 1$$



$$f(x) = -2\sin(-2x+1) + \sin(-x+2) - \cos(-2x+2) - 2\cos(-2x) + \cos(2x) + 1.$$



$$f(x) = -2\sin(-x) - \cos(-3x+1) - \cos(x+1) + 1.$$



$$f(x) = -\sin(3x+1) + \sin(-x) + \sin(2x) + \sin(3x) - \cos(x+1) + 1.$$



$$f(x) = \sin(x+1) - 2\sin(x) - \cos(-x+1) - \cos(x+1) + 2\cos(2x) + 1$$



$$f(x) = \sin(-3x+1) - \cos(-3x+1) + \cos(x+2) + \cos(-2x) - 2\cos(2x) + 1.$$



$$f(x) = -\sin(x+1) + \sin(-x) + 2\sin(x) + \cos(-x+1) + \cos(2x) + 1.$$



$$f(x) = -\sin(2x+1) - \sin(-2x) + \cos(-3x+1) - \cos(x+1) + 2\cos(3x+2) + 1.$$


$$f(x) = -2\sin(-2x+2) - 2\sin(-x+2) + \sin(2x+1) + 2\sin(2x+2) + \cos(-2x+2) + 1$$



$$f(x) = 2\sin(x+1) + \sin(3x+2) + \cos(-x) + 1.$$



$$f(x) = -\sin\left(-x+2\right) + 2\,\sin\left(3\,x\right) - 2\,\cos\left(-3\,x+1\right) + 1.$$



$$f(x) = \sin(2x+2) - 2\sin(x) + \cos(-x+2) + \cos(3x+2) - 2\cos(x) + 1$$



$$f(x) = -\sin(-x+2) - 2\sin(x+2) + \cos(-2x+1) + 2\cos(-x+1) - 2\cos(-x) + 1.$$



$$f(x) = -2\sin(-x+2) - \sin(-2x) - \sin(3x) + \cos(-2x) + 2\cos(-x) + 1$$



$$f(x) = -\sin(-2x+1) + \sin(2x) - \cos(-x) + 1.$$



$$f(x) = \sin(-x+1) - \cos(-2x+1) - \cos(-x+1) - \cos(x) + 1.$$



$$f(x) = \sin\left(-2x+2\right) + \cos\left(-2x+2\right) + \cos\left(3x+1\right) - \cos\left(-2x\right) + 1.$$



$$f(x) = 2\sin(-2x+1) - \sin(2x+2) - 2\cos(-x+1) + \cos(-3x) + 1.$$



$$f(x) = \sin(3x+2) + \sin(-2x) + 2\sin(x) - \cos(-3x) + 1.$$



$$f(x) = 2\sin(-x+2) + 2\sin(x+1) + \sin(3x+2) + 2\cos(x+1) + 1.$$



$$f(x) = \sin(-x+1) + \sin(2x+1) + \sin(-3x) + 2\cos(-3x+2) - 2\cos(x+1) + 1$$



$$f(x) = -\sin(3x+2) - 2\sin(-3x) - 2\cos(-3x+2) - \cos(-x+2) + \cos(-x) + 1$$



$$f(x) = -\sin(-3x+2) - \sin(x) - 2\cos(-3x) - \cos(-2x) + 2\cos(3x) + 1.$$



$$f(x) = \sin(-3x+1) - \sin(-2x) + \cos(2x+1) - 2\cos(x) + 1$$



$$f(x) = 2\sin(x+1) - \sin(x+2) - 2\cos(2x) + 1$$



$$f(x) = -2\sin(-x+1) + 2\sin(x+2) + 2\sin(3x+2) + 2\cos(-3x+2) - 2\cos(-x+2) + 1$$



$$f(x) = \sin(x+1) - \cos(-3x+1) - \cos(-x+2) + 2\cos(-3x) - \cos(x) + 1.$$



$$f(x) = -\sin(-3x+2) + \sin(-x+1) - \cos(x+2) - \cos(-3x) - \cos(x) + 1.$$



$$f(x) = 2\sin(x+1) + \sin(2x+1) + 2\sin(x) + 2\cos(2x+2) - 2\cos(x) + 1.$$



$$f(x) = -\sin(-x+1) + 2\sin(x+2) + \sin(3x+1) + \sin(3x) + \sin(x) + 1.$$



$$f(x) = 2\sin(x) - \cos(-x+2) - \cos(x+1) + 1.$$



$$f(x) = -2\sin(x+1) + \sin(x) + 2\cos(-x+1) + \cos(-2x) + \cos(-x) + 1.$$



$$f(x) = -\sin(-2x+2) + 2\cos(-2x+1) - \cos(-2x+2) - \cos(-3x) - \cos(-2x) + 1.$$



$$f(x) = 2\sin(x+2) + \sin(-2x) - \sin(2x) + 2\cos(-2x+1) - 2\cos(x) + 1.$$



$$f(x) = 2\sin(-2x+1) + \cos(-2x+2) + \cos(-x+2) - \cos(3x+1) + \cos(3x) + 1$$

